cava/arrow-examples/Aes/Pkg.v
@@ -8,43 +8,37 @@ Import KappaNotation.
 Require Import Util List.
 
 Section var.
-Variable var: Kind -> Kind -> Type.
+  Context {var: Kind -> Kind -> Type}.
 
-(* typedef enum logic {
-  CIPH_FWD = 1'b0,
-  CIPH_INV = 1'b1
-} ciph_op_e; *)
-Definition CIPH_FWD {n} : kappa_sugared var Unit (Vector n Bit) := <[ #0 ]>.
-Definition CIPH_INV {n} : kappa_sugared var Unit (Vector n Bit) := <[ #1 ]>.
+  (* typedef enum logic {
+    CIPH_FWD = 1'b0,
+    CIPH_INV = 1'b1
+  } ciph_op_e; *)
+  Definition CIPH_FWD {n} : kappa_sugared var Unit (Vector n Bit) := <[ #0 ]>.
+  Definition CIPH_INV {n} : kappa_sugared var Unit (Vector n Bit) := <[ #1 ]>.
 
-Fixpoint outer {n}
-  : kappa_sugared var <<Bit, Unit>> (Vector (S n) Bit) := 
-match n with
-| 0 => <[ \x => mkVec (x) ]>
-| S n => <[ \x => x :: !outer x ]>
-end.
+  Fixpoint outer {n}
+    : kappa_sugared var <<Bit, Unit>> (Vector (S n) Bit) := 
+  match n with
+  | 0 => <[ \x => mkVec (x) ]>
+  | S n => <[ \x => x :: !outer x ]>
+  end.
 
-Definition aes_mvm_acc
-  : kappa_sugared var <<Vector 8 Bit, Vector 8 Bit, Bit, Unit>> (Vector 8 Bit) := 
-  <[\acc mat vec => acc ^ (mat & (!outer vec)) ]>.
+  Definition aes_mvm_acc
+    : kappa_sugared var <<Vector 8 Bit, Vector 8 Bit, Bit, Unit>> (Vector 8 Bit) := 
+    <[\acc mat vec => acc ^ (mat & (!outer vec)) ]>.
 
-Definition aes_mvm: kappa_sugared var <<Vector 8 Bit, Vector 8 (Vector 8 Bit), Unit>> (Vector 8 Bit) :=
-  <[\ vec_b mat_a =>
-  let _1 = !aes_mvm_acc (#0) (mat_a[#0]) (vec_b[#7]) in
-  let _2 = !aes_mvm_acc (_1) (mat_a[#1]) (vec_b[#6]) in
-  let _3 = !aes_mvm_acc (_2) (mat_a[#2]) (vec_b[#5]) in
-  let _4 = !aes_mvm_acc (_3) (mat_a[#3]) (vec_b[#4]) in
-  let _5 = !aes_mvm_acc (_4) (mat_a[#4]) (vec_b[#3]) in
-  let _6 = !aes_mvm_acc (_5) (mat_a[#5]) (vec_b[#2]) in
-  let _7 = !aes_mvm_acc (_6) (mat_a[#6]) (vec_b[#1]) in
-  let _8 = !aes_mvm_acc (_7) (mat_a[#7]) (vec_b[#0]) in
-  _8
-  ]>.
+  Definition aes_mvm: kappa_sugared var <<Vector 8 Bit, Vector 8 (Vector 8 Bit), Unit>> (Vector 8 Bit) :=
+    <[\ vec_b mat_a =>
+    let _1 = !aes_mvm_acc (#0) (mat_a[#0]) (vec_b[#7]) in
+    let _2 = !aes_mvm_acc (_1) (mat_a[#1]) (vec_b[#6]) in
+    let _3 = !aes_mvm_acc (_2) (mat_a[#2]) (vec_b[#5]) in
+    let _4 = !aes_mvm_acc (_3) (mat_a[#3]) (vec_b[#4]) in
+    let _5 = !aes_mvm_acc (_4) (mat_a[#4]) (vec_b[#3]) in
+    let _6 = !aes_mvm_acc (_5) (mat_a[#5]) (vec_b[#2]) in
+    let _7 = !aes_mvm_acc (_6) (mat_a[#6]) (vec_b[#1]) in
+    let _8 = !aes_mvm_acc (_7) (mat_a[#7]) (vec_b[#0]) in
+    _8
+    ]>.
 
 End var.
-
-
-Arguments aes_mvm {var}. 
-Arguments outer {var}. 
-Arguments CIPH_FWD {var n}. 
-Arguments CIPH_INV {var n}. 
