cava/arrow-examples/Aes/canright_masked_noreuse.v
@@ -13,193 +13,193 @@ Require Import pkg.
 Require Import canright_pkg.
 
 Section var.
-Variable var: Kind -> Kind -> Type.
+  Context {var: Kind -> Kind -> Type}.
 
-(* function automatic logic [3:0] aes_masked_inverse_gf2p4(logic [3:0] b,
-                                                        logic [3:0] q,
-                                                        logic [1:0] r,
-                                                        logic [3:0] t);*)
-Definition aes_masked_inverse_gf2p4
-  : kappa_sugared var
-    << Vector 4 Bit (* b *)
-    ,  Vector 4 Bit (* q *)
-    ,  Vector 2 Bit (* r *)
-    ,  Vector 4 Bit (* t *)
-    ,  Unit >> 
-    <<Vector 4 Bit>>. refine (
-<[ \b q r t =>
-    let b1 = b[3:2] in
-    let b0 = b[1:0] in
-    let q1 = q[3:2] in
-    let q0 = q[1:0] in
-    let t1 = t[3:2] in
-    let t0 = t[1:0] in
+  (* function automatic logic [3:0] aes_masked_inverse_gf2p4(logic [3:0] b,
+                                                          logic [3:0] q,
+                                                          logic [1:0] r,
+                                                          logic [3:0] t);*)
+  Definition aes_masked_inverse_gf2p4
+    : kappa_sugared var
+      << Vector 4 Bit (* b *)
+      ,  Vector 4 Bit (* q *)
+      ,  Vector 2 Bit (* r *)
+      ,  Vector 4 Bit (* t *)
+      ,  Unit >> 
+      <<Vector 4 Bit>>. refine (
+  <[ \b q r t =>
+      let b1 = b[3:2] in
+      let b0 = b[1:0] in
+      let q1 = q[3:2] in
+      let q0 = q[1:0] in
+      let t1 = t[3:2] in
+      let t0 = t[1:0] in
 
-    (* // Formula 13
-    // IMPORTANT: The following ops must be executed in order (left to right):
-    c = r ^ aes_scale_omega2_gf2p2(aes_square_gf2p2(b1 ^ b0))
-          ^ aes_scale_omega2_gf2p2(aes_square_gf2p2(q1 ^ q0))
-          ^ aes_mul_gf2p2(b1, b0)
-          ^ aes_mul_gf2p2(b1, q0) ^ aes_mul_gf2p2(b0, q1) ^ aes_mul_gf2p2(q1, q0); *)
-    let temp1 = !aes_scale_omega2_gf2p2 (!aes_square_gf2p2 (b1 ^ b0)) in
-    let temp2 = !aes_scale_omega2_gf2p2 (!aes_square_gf2p2 (q1 ^ q0)) in 
-    let temp3 = !aes_mul_gf2p2 b1 b0 in 
-    let temp4 = !aes_mul_gf2p2 b1 q0 ^ !aes_mul_gf2p2 b0 q1 ^ !aes_mul_gf2p2 q1 q0 in
+      (* // Formula 13
+      // IMPORTANT: The following ops must be executed in order (left to right):
+      c = r ^ aes_scale_omega2_gf2p2(aes_square_gf2p2(b1 ^ b0))
+            ^ aes_scale_omega2_gf2p2(aes_square_gf2p2(q1 ^ q0))
+            ^ aes_mul_gf2p2(b1, b0)
+            ^ aes_mul_gf2p2(b1, q0) ^ aes_mul_gf2p2(b0, q1) ^ aes_mul_gf2p2(q1, q0); *)
+      let temp1 = !aes_scale_omega2_gf2p2 (!aes_square_gf2p2 (b1 ^ b0)) in
+      let temp2 = !aes_scale_omega2_gf2p2 (!aes_square_gf2p2 (q1 ^ q0)) in 
+      let temp3 = !aes_mul_gf2p2 b1 b0 in 
+      let temp4 = !aes_mul_gf2p2 b1 q0 ^ !aes_mul_gf2p2 b0 q1 ^ !aes_mul_gf2p2 q1 q0 in
 
-    let c = r ^ temp1 ^ temp2 ^ temp3 ^ temp4 in
+      let c = r ^ temp1 ^ temp2 ^ temp3 ^ temp4 in
 
-    (* // Formulas 14 and 15
-    c_inv = aes_square_gf2p2(c);
-    r_sq  = aes_square_gf2p2(r); *)
+      (* // Formulas 14 and 15
+      c_inv = aes_square_gf2p2(c);
+      r_sq  = aes_square_gf2p2(r); *)
 
-    let c_inv = !aes_square_gf2p2 c in
-    let r_sq  = !aes_square_gf2p2 r in
+      let c_inv = !aes_square_gf2p2 c in
+      let r_sq  = !aes_square_gf2p2 r in
 
-    (* // Formulas 16 and 17
-    // IMPORTANT: The following ops must be executed in order (left to right):
-    b1_inv = t1 ^ aes_mul_gf2p2(b0, c_inv)
-                ^ aes_mul_gf2p2(b0, r_sq) ^ aes_mul_gf2p2(q0, c_inv) ^ aes_mul_gf2p2(q0, r_sq);
-    b0_inv = t0 ^ aes_mul_gf2p2(b1, c_inv)
-                ^ aes_mul_gf2p2(b1, r_sq) ^ aes_mul_gf2p2(q1, c_inv) ^ aes_mul_gf2p2(q1, r_sq);
-    // *)
+      (* // Formulas 16 and 17
+      // IMPORTANT: The following ops must be executed in order (left to right):
+      b1_inv = t1 ^ aes_mul_gf2p2(b0, c_inv)
+                  ^ aes_mul_gf2p2(b0, r_sq) ^ aes_mul_gf2p2(q0, c_inv) ^ aes_mul_gf2p2(q0, r_sq);
+      b0_inv = t0 ^ aes_mul_gf2p2(b1, c_inv)
+                  ^ aes_mul_gf2p2(b1, r_sq) ^ aes_mul_gf2p2(q1, c_inv) ^ aes_mul_gf2p2(q1, r_sq);
+      // *)
 
-    let b1_inv = t1 ^ !aes_mul_gf2p2 b0 c_inv
-                    ^ !aes_mul_gf2p2 b0 r_sq ^ !aes_mul_gf2p2 q0 c_inv ^ !aes_mul_gf2p2 q0 r_sq in
-    let b0_inv = t0 ^ !aes_mul_gf2p2 b1 c_inv
-                    ^ !aes_mul_gf2p2 b1 r_sq ^ !aes_mul_gf2p2 q1 c_inv ^ !aes_mul_gf2p2 q1 r_sq in
+      let b1_inv = t1 ^ !aes_mul_gf2p2 b0 c_inv
+                      ^ !aes_mul_gf2p2 b0 r_sq ^ !aes_mul_gf2p2 q0 c_inv ^ !aes_mul_gf2p2 q0 r_sq in
+      let b0_inv = t0 ^ !aes_mul_gf2p2 b1 c_inv
+                      ^ !aes_mul_gf2p2 b1 r_sq ^ !aes_mul_gf2p2 q1 c_inv ^ !aes_mul_gf2p2 q1 r_sq in
 
-    (* // Note: b_inv is masked by t, b was masked by q.
-    b_inv = {b1_inv, b0_inv}; *)
+      (* // Note: b_inv is masked by t, b was masked by q.
+      b_inv = {b1_inv, b0_inv}; *)
 
-    concat b0_inv b1_inv
+      concat b0_inv b1_inv
 
-]>); lia.
-Defined.
+  ]>); lia.
+  Defined.
 
-Definition aes_masked_inverse_gf2p8
-  : kappa_sugared var
-    << Vector 8 Bit (* a *)
-    ,  Vector 8 Bit (* m *)
-    ,  Vector 8 Bit (* n *)
-    ,  Unit >> 
-    <<Vector 8 Bit>>. refine (
-<[ \a m n =>
-    let a1 = a[7:4] in
-    let a0 = a[3:0] in
-    let m1 = m[7:4] in
-    let m0 = m[3:0] in
+  Definition aes_masked_inverse_gf2p8
+    : kappa_sugared var
+      << Vector 8 Bit (* a *)
+      ,  Vector 8 Bit (* m *)
+      ,  Vector 8 Bit (* n *)
+      ,  Unit >> 
+      <<Vector 8 Bit>>. refine (
+  <[ \a m n =>
+      let a1 = a[7:4] in
+      let a0 = a[3:0] in
+      let m1 = m[7:4] in
+      let m0 = m[3:0] in
 
-    (* // q must be independent of m. *)
-    let q = n[7:4] in
+      (* // q must be independent of m. *)
+      let q = n[7:4] in
 
-    (* // Formula 12
-    // IMPORTANT: The following ops must be executed in order (left to right):
-    b = q ^ aes_square_scale_gf2p4_gf2p2(a1 ^ a0)
-          ^ aes_square_scale_gf2p4_gf2p2(m1 ^ m0)
-          ^ aes_mul_gf2p4(a1, a0)
-          ^ aes_mul_gf2p4(a1, m0) ^ aes_mul_gf2p4(a0, m1) ^ aes_mul_gf2p4(m1, m0); *)
-    
-    let b = q ^ !aes_square_scale_gf2p4_gf2p2 (a1 ^ a0)
-              ^ !aes_square_scale_gf2p4_gf2p2 (m1 ^ m0)
-              ^ !aes_mul_gf2p4 a1 a0
-              ^ !aes_mul_gf2p4 a1 m0 ^ !aes_mul_gf2p4 a0 m1 ^ !aes_mul_gf2p4 m1 m0 in
+      (* // Formula 12
+      // IMPORTANT: The following ops must be executed in order (left to right):
+      b = q ^ aes_square_scale_gf2p4_gf2p2(a1 ^ a0)
+            ^ aes_square_scale_gf2p4_gf2p2(m1 ^ m0)
+            ^ aes_mul_gf2p4(a1, a0)
+            ^ aes_mul_gf2p4(a1, m0) ^ aes_mul_gf2p4(a0, m1) ^ aes_mul_gf2p4(m1, m0); *)
+      
+      let b = q ^ !aes_square_scale_gf2p4_gf2p2 (a1 ^ a0)
+                ^ !aes_square_scale_gf2p4_gf2p2 (m1 ^ m0)
+                ^ !aes_mul_gf2p4 a1 a0
+                ^ !aes_mul_gf2p4 a1 m0 ^ !aes_mul_gf2p4 a0 m1 ^ !aes_mul_gf2p4 m1 m0 in
 
-    (* // r must be independent of q. *)
-    let r = m1[3:2] in
+      (* // r must be independent of q. *)
+      let r = m1[3:2] in
 
-    (* // Note that the paper states the following requirements on t:
-    // - t must be independent of r.
-    // - t1 must be independent of q0, t0 must be independent of q1.
-    // - t must be independent of m (for the final steps involving s)
-    // The paper suggests to use t = q. To select s = n for the output mask (s must be independent
-    // of t = q = n[7:4]), we would need t = m0 or similar (not r, m1[3:2] though), but this would
-    // break the random product distribution of aes_mul_gf2p4(m0, t), or aes_mul_gf2p4(m1, t) below
-    // (see Lemma 2 in the paper). For this reason, we select t = q here and apply a final mask
-    // switch from s = m to n after the inversion.
-    t = q; *)
-    let t = q in
+      (* // Note that the paper states the following requirements on t:
+      // - t must be independent of r.
+      // - t1 must be independent of q0, t0 must be independent of q1.
+      // - t must be independent of m (for the final steps involving s)
+      // The paper suggests to use t = q. To select s = n for the output mask (s must be independent
+      // of t = q = n[7:4]), we would need t = m0 or similar (not r, m1[3:2] though), but this would
+      // break the random product distribution of aes_mul_gf2p4(m0, t), or aes_mul_gf2p4(m1, t) below
+      // (see Lemma 2 in the paper). For this reason, we select t = q here and apply a final mask
+      // switch from s = m to n after the inversion.
+      t = q; *)
+      let t = q in
 
-    (* // b is masked by q, b_inv is masked by t. *)
-    let b_inv = !aes_masked_inverse_gf2p4 b q r t in
+      (* // b is masked by q, b_inv is masked by t. *)
+      let b_inv = !aes_masked_inverse_gf2p4 b q r t in
 
-    (* // Note that the paper states the following requirements on s:
-    // - s must be independent of t
-    // - s1 must be independent of m0, s0 must be independent of m1.
-    // The paper suggests to use s = m (the input mask). To still end up with the specified output
-    // mask n, we will apply a final mask switch after the inversion.
-    s1 = m1;
-    s0 = m0; *)
-    let s1 = m1 in
-    let s0 = m0 in
+      (* // Note that the paper states the following requirements on s:
+      // - s must be independent of t
+      // - s1 must be independent of m0, s0 must be independent of m1.
+      // The paper suggests to use s = m (the input mask). To still end up with the specified output
+      // mask n, we will apply a final mask switch after the inversion.
+      s1 = m1;
+      s0 = m0; *)
+      let s1 = m1 in
+      let s0 = m0 in
 
-    (* // Formulas 18 and 19
-    // IMPORTANT: The following ops must be executed in order (left to right):
-    a1_inv = s1 ^ aes_mul_gf2p4(a0, b_inv)
-                ^ aes_mul_gf2p4(a0, t) ^ aes_mul_gf2p4(m0, b_inv) ^ aes_mul_gf2p4(m0, t);
-    a0_inv = s0 ^ aes_mul_gf2p4(a1, b_inv)
-                ^ aes_mul_gf2p4(a1, t) ^ aes_mul_gf2p4(m1, b_inv) ^ aes_mul_gf2p4(m1, t);
-    // *)
-    let a1_inv = s1 ^ !aes_mul_gf2p4 a0 b_inv
-                    ^ !aes_mul_gf2p4 a0 t ^ !aes_mul_gf2p4 m0 b_inv ^ !aes_mul_gf2p4 m0 t in
-    let a0_inv = s0 ^ !aes_mul_gf2p4 a1 b_inv
-                    ^ !aes_mul_gf2p4 a1 t ^ !aes_mul_gf2p4 m1 b_inv ^ !aes_mul_gf2p4 m1 t in
+      (* // Formulas 18 and 19
+      // IMPORTANT: The following ops must be executed in order (left to right):
+      a1_inv = s1 ^ aes_mul_gf2p4(a0, b_inv)
+                  ^ aes_mul_gf2p4(a0, t) ^ aes_mul_gf2p4(m0, b_inv) ^ aes_mul_gf2p4(m0, t);
+      a0_inv = s0 ^ aes_mul_gf2p4(a1, b_inv)
+                  ^ aes_mul_gf2p4(a1, t) ^ aes_mul_gf2p4(m1, b_inv) ^ aes_mul_gf2p4(m1, t);
+      // *)
+      let a1_inv = s1 ^ !aes_mul_gf2p4 a0 b_inv
+                      ^ !aes_mul_gf2p4 a0 t ^ !aes_mul_gf2p4 m0 b_inv ^ !aes_mul_gf2p4 m0 t in
+      let a0_inv = s0 ^ !aes_mul_gf2p4 a1 b_inv
+                      ^ !aes_mul_gf2p4 a1 t ^ !aes_mul_gf2p4 m1 b_inv ^ !aes_mul_gf2p4 m1 t in
 
-    (* // Note: a_inv is now masked by s = m, a was masked by m. *)
-    let a_inv = concat a0_inv a1_inv in
+      (* // Note: a_inv is now masked by s = m, a was masked by m. *)
+      let a_inv = concat a0_inv a1_inv in
 
-    (* // To have a_inv masked by n (the specified output mask), we perform a final mask switch.
-    // IMPORTANT: The following ops must be executed in order (left to right):
-    a_inv = a_inv ^ n ^ m; *)
-    let a_inv' = a_inv ^ n ^ m in
+      (* // To have a_inv masked by n (the specified output mask), we perform a final mask switch.
+      // IMPORTANT: The following ops must be executed in order (left to right):
+      a_inv = a_inv ^ n ^ m; *)
+      let a_inv' = a_inv ^ n ^ m in
 
-    a_inv'
-]>); lia.
-Defined.
+      a_inv'
+  ]>); lia.
+  Defined.
 
-Definition aes_sbox_canright_masked_noreuse
-  : kappa_sugared var << 
-    Vector 1 Bit, (* TODO: wrapped type?  aes_pkg::ciph_op_e op_i, *)
+  Definition aes_sbox_canright_masked_noreuse
+    : kappa_sugared var << 
+      Vector 1 Bit, (* TODO: wrapped type?  aes_pkg::ciph_op_e op_i, *)
 
-    Vector 8 Bit, (* data_i, // masked, the actual input data is data_i ^ in_mask_i *)
-    Vector 8 Bit, (* in_mask_i,  // input mask, independent from actual input data *)
-    Vector 8 Bit, (* out_mask_i, // output mask, independent from input mask *)
-    Unit >> << Vector 8 Bit>> :=
-<[ \op_i data_i in_mask_i out_mask_i =>
-    (* // Convert data to normal basis X.
-    assign data_basis_x = (op_i == CIPH_FWD) ? aes_mvm(data_i, A2X) :
-                                              aes_mvm(data_i ^ 8'h63, S2X); *)
-    let data_basis_x = if op_i == !CIPH_FWD
-                       then !aes_mvm data_i !A2X
-                       else !aes_mvm (data_i ^ #99) !S2X in
+      Vector 8 Bit, (* data_i, // masked, the actual input data is data_i ^ in_mask_i *)
+      Vector 8 Bit, (* in_mask_i,  // input mask, independent from actual input data *)
+      Vector 8 Bit, (* out_mask_i, // output mask, independent from input mask *)
+      Unit >> << Vector 8 Bit>> :=
+  <[ \op_i data_i in_mask_i out_mask_i =>
+      (* // Convert data to normal basis X.
+      assign data_basis_x = (op_i == CIPH_FWD) ? aes_mvm(data_i, A2X) :
+                                                aes_mvm(data_i ^ 8'h63, S2X); *)
+      let data_basis_x = if op_i == !CIPH_FWD
+                        then !aes_mvm data_i !A2X
+                        else !aes_mvm (data_i ^ #99) !S2X in
 
-    (* // Convert masks to normal basis X.
-    // The addition of constant 8'h63 following the affine transformation is skipped.
-    assign in_mask_basis_x  = (op_i == CIPH_FWD) ? aes_mvm(in_mask_i, A2X) :
-                                                  aes_mvm(in_mask_i, S2X); *)
-    let in_mask_basis_x = if op_i == !CIPH_FWD
-                          then !aes_mvm in_mask_i !A2X 
-                          else !aes_mvm in_mask_i !S2X in
+      (* // Convert masks to normal basis X.
+      // The addition of constant 8'h63 following the affine transformation is skipped.
+      assign in_mask_basis_x  = (op_i == CIPH_FWD) ? aes_mvm(in_mask_i, A2X) :
+                                                    aes_mvm(in_mask_i, S2X); *)
+      let in_mask_basis_x = if op_i == !CIPH_FWD
+                            then !aes_mvm in_mask_i !A2X 
+                            else !aes_mvm in_mask_i !S2X in
 
-    (* // The output mask is converted in the opposite direction.
-    assign out_mask_basis_x = (op_i == CIPH_INV) ? aes_mvm(out_mask_i, A2X) :
-                                                  aes_mvm(out_mask_i, S2X); *)
-    let out_mask_basis_x = if op_i == !CIPH_INV
-                           then !aes_mvm out_mask_i !A2X
-                           else !aes_mvm out_mask_i !S2X in
+      (* // The output mask is converted in the opposite direction.
+      assign out_mask_basis_x = (op_i == CIPH_INV) ? aes_mvm(out_mask_i, A2X) :
+                                                    aes_mvm(out_mask_i, S2X); *)
+      let out_mask_basis_x = if op_i == !CIPH_INV
+                            then !aes_mvm out_mask_i !A2X
+                            else !aes_mvm out_mask_i !S2X in
 
-    (* // Do the inversion in normal basis X.
-    assign data_inverse = aes_masked_inverse_gf2p8(data_basis_x, in_mask_basis_x, out_mask_basis_x); *)
-    let data_inverse = !aes_masked_inverse_gf2p8 data_basis_x in_mask_basis_x out_mask_basis_x in
+      (* // Do the inversion in normal basis X.
+      assign data_inverse = aes_masked_inverse_gf2p8(data_basis_x, in_mask_basis_x, out_mask_basis_x); *)
+      let data_inverse = !aes_masked_inverse_gf2p8 data_basis_x in_mask_basis_x out_mask_basis_x in
 
-    (* // Convert to basis S or A.
-    assign data_o = (op_i == CIPH_FWD) ? (aes_mvm(data_inverse, X2S) ^ 8'h63) :
-                                        (aes_mvm(data_inverse, X2A)); *)
-    let data_o = if op_i == !CIPH_FWD
-                 then !aes_mvm data_inverse !X2S ^ #99
-                 else !aes_mvm data_inverse !X2A
-                 in
+      (* // Convert to basis S or A.
+      assign data_o = (op_i == CIPH_FWD) ? (aes_mvm(data_inverse, X2S) ^ 8'h63) :
+                                          (aes_mvm(data_inverse, X2A)); *)
+      let data_o = if op_i == !CIPH_FWD
+                  then !aes_mvm data_inverse !X2S ^ #99
+                  else !aes_mvm data_inverse !X2A
+                  in
 
-    data_o
-]>.
+      data_o
+  ]>.
 
 End var.
